Lots of progress on SmallStep

SoftwareFoundations/ProgrammingLanguageFoundations/SmallStep.lean
@@ -2,6 +2,8 @@
 # Small-Step Operational Semantics
 -/
 
+import SoftwareFoundations.LogicalFoundations.Imp
+
 namespace SoftwareFoundations.ProgrammingLanguageFoundations.SmallStep
   /-
   ## A Toy Language
@@ -97,8 +99,8 @@ namespace SoftwareFoundations.ProgrammingLanguageFoundations.SmallStep
             _ = Term.plus _ _ := congrFun (congrArg Term.plus ih) _
         | _, _, _, .plusR h₁, .plusR h₂ =>
           have ih := deterministic h₁ h₂
-          calc Term.plus (.const _) _
-            _ = Term.plus (.const _) _ := congrArg (Term.plus (.const _)) ih
+          calc Term.plus _ _
+            _ = Term.plus _ _ := congrArg (Term.plus _) ih
     end Term
 
     namespace Tactic
@@ -140,13 +142,11 @@ namespace SoftwareFoundations.ProgrammingLanguageFoundations.SmallStep
         have ih := deterministic h₁ h₂
         calc Term.plus _ _
           _ = Term.plus _ _ := congrFun (congrArg Term.plus ih) _
-      | _, _, _, .plusR hv h₁, .plusL h₂ =>
-        sorry
-      | _, _, _, .plusR hv₁ h₁, .plusR hv₂ h₂ =>
+      | _, _, _, .plusR (.const _) h₁, .plusL h₂ => sorry
+      | _, _, _, .plusR _ h₁, .plusR _ h₂ =>
         have ih := deterministic h₁ h₂
-        -- calc Term.plus (.const _) _
-        --   _ = Term.plus (.const _) _ := congrArg (Term.plus (.const _)) ih
-        sorry
+        calc Term.plus _ _
+          _ = Term.plus _ _ := congrArg (Term.plus _) ih
   end Term
 
   namespace Tactic
@@ -155,18 +155,22 @@ namespace SoftwareFoundations.ProgrammingLanguageFoundations.SmallStep
       intro h₁ h₂
       cases h₁ <;> cases h₂ <;> try (first | rfl
                                            | contradiction)
-      case plusL.plusL _ _ _ h₁ _ h₂       => rw [deterministic h₁ h₂]
-      case plusR.plusR _ _ hv₁ h₁ _ hv₂ h₂ => rw [deterministic h₁ h₂]
-      case plusL.plusR _ _ _ h₁ _ hv h₂    => sorry
-      case plusR.plusL _ _ _ hv h₁ _ h₂    => sorry
+      case plusL.plusL _ _ _ h₁ _ h₂    => rw [deterministic h₁ h₂]
+      case plusR.plusR _ _ _ h₁ _ _ h₂  => rw [deterministic h₁ h₂]
+      case plusL.plusR _ _ _ h₁ _ hv h₂ =>
+        cases hv with
+          | const => contradiction
+      case plusR.plusL _ _ _ hv h₁ _ h₂ =>
+        cases hv with
+          | const => contradiction
   end Tactic
 
   namespace Blended
     theorem Eval₁.deterministic: Relation.deterministic Eval₁
-      | _, _, _, .constConst, .constConst => by rfl
-      | _, _, _, .plusL h₁, .plusL h₂ => by rw [deterministic h₁ h₂]
-      | _, _, _, .plusR hv₁ h₁, .plusR hv₂ h₂ => by rw [deterministic h₁ h₂]
-      | _, _, _, .plusR hv h₁, .plusL h₂ => sorry
+      | _, _, _, .constConst, .constConst       => by rfl
+      | _, _, _, .plusL h₁, .plusL h₂           => by rw [deterministic h₁ h₂]
+      | _, _, _, .plusR _ h₁, .plusR _ h₂       => by rw [deterministic h₁ h₂]
+      | _, _, _, .plusR (.const _) _, .plusL h₂ => by contradiction
   end Blended
 
   /-
@@ -194,19 +198,21 @@ namespace SoftwareFoundations.ProgrammingLanguageFoundations.SmallStep
           cases ih₁ with
             | inr ex =>
               apply Or.inr
-              · apply Exists.intro
-                · apply Eval₁.plusL
-                  · sorry
-                  · sorry
+              cases ex with
+                | intro w hw =>
+                  exists (.plus w t₂)
+                  · apply Eval₁.plusL
+                    · exact hw
             | inl hv₁ =>
               cases ih₂ with
                 | inr ex =>
                   apply Or.inr
-                  · apply Exists.intro
-                    · apply Eval₁.plusR
-                      · exact hv₁
-                      · sorry
-                      · sorry
+                  cases ex with
+                    | intro w hw =>
+                      exists (.plus t₁ w)
+                      · apply Eval₁.plusR
+                        · exact hv₁
+                        · exact hw
                 | inl hv₂ =>
                   cases t₁ with
                     | plus _ _ => contradiction
@@ -454,10 +460,10 @@ namespace SoftwareFoundations.ProgrammingLanguageFoundations.SmallStep
         | .true => .inl .true
         | .false => .inl .false
         | .test c t f =>
-          match strong_progress c, strong_progress t, strong_progress f with
-            | .inl .true, _, _ => .inr ⟨[TF| ‹t›], .testTrue⟩
-            | .inl .false, _, _ => .inr ⟨[TF| ‹f›], .testFalse⟩
-            | .inr ⟨w, hw⟩, _, _ => .inr ⟨[TF| test (‹w›) { ‹t›} else { ‹f› }], .test hw⟩
+          match strong_progress c with
+            | .inl .true   => .inr ⟨[TF| ‹t›], .testTrue⟩
+            | .inl .false  => .inr ⟨[TF| ‹f›], .testFalse⟩
+            | .inr ⟨w, hw⟩ => .inr ⟨[TF| test (‹w›) { ‹t› } else { ‹f› }], .test hw⟩
 
       theorem Eval₁.deterministic: Relation.deterministic Eval₁
         | _, _, _, .testTrue, .testTrue
@@ -465,11 +471,37 @@ namespace SoftwareFoundations.ProgrammingLanguageFoundations.SmallStep
         | _, _, _, .test h₁, .test h₂ =>
           have ih := deterministic h₁ h₂
           calc Term.test _ _ _
-            _ = Term.test _ _ _ := by rw [ih] -- TODO: Remove Tactic Block
+            _ = Term.test _ _ _ := congrFun (congrFun (congrArg Term.test ih) _) _
     end Term
 
     namespace Tactic
-      theorem Eval₁.strong_progress: ∀ t₁: Term, Value t₁ ∨ ∃ t₂: Term, Eval₁ t₁ t₂ := sorry
+      theorem Eval₁.strong_progress (t₁: Term): Value t₁ ∨ ∃ t₂: Term, Eval₁ t₁ t₂ := by
+        induction t₁ with
+          | true =>
+            apply Or.inl
+            · apply Value.true
+          | false =>
+            apply Or.inl
+            · apply Value.false
+          | «test» c t f ih =>
+            cases ih with
+              | inl v =>
+                cases v with
+                  | true =>
+                    apply Or.inr
+                    · exists [TF| ‹t›]
+                      · apply Eval₁.testTrue
+                  | false =>
+                    apply Or.inr
+                    · exists [TF| ‹f›]
+                      · apply Eval₁.testFalse
+              | inr ex =>
+                cases ex with
+                  | intro w hw =>
+                    apply Or.inr
+                    · exists [TF| test (‹w›) { ‹t› } else { ‹f› }]
+                      · apply Eval₁.test
+                        · exact hw
 
       theorem Eval₁.deterministic: Relation.deterministic Eval₁ := by
         intro _ _ _ h₁ h₂
@@ -483,10 +515,10 @@ namespace SoftwareFoundations.ProgrammingLanguageFoundations.SmallStep
         | .true => .inl .true
         | .false => .inl .false
         | .test c t f =>
-          match strong_progress c, strong_progress t, strong_progress f with
-            | .inl .true, _, _ => .inr ⟨[TF| ‹t›], .testTrue⟩
-            | .inl .false, _, _ => .inr ⟨[TF| ‹f›], .testFalse⟩
-            | .inr ⟨w, hw⟩, _, _ => .inr ⟨[TF| test (‹w›) { ‹t›} else { ‹f› }], .test hw⟩
+          match strong_progress c with
+            | .inl .true   => .inr ⟨[TF| ‹t›], .testTrue⟩
+            | .inl .false  => .inr ⟨[TF| ‹f›], .testFalse⟩
+            | .inr ⟨w, hw⟩ => .inr ⟨[TF| test (‹w›) { ‹t›} else { ‹f› }], .test hw⟩
 
       theorem Eval₁.deterministic: Relation.deterministic Eval₁
         | _, _, _, .testTrue, .testTrue => rfl
@@ -499,7 +531,7 @@ namespace SoftwareFoundations.ProgrammingLanguageFoundations.SmallStep
         | testTrue {t f: Term}: Eval₁ [TF| test (tru) { ‹t› } else { ‹f› }] t
         | testFalse {t f: Term}: Eval₁ [TF| test (fls) { ‹t› } else { ‹f› }] f
         | test {c₁ c₂ t f: Term} (h: Eval₁ c₁ c₂): Eval₁ [TF| test (‹c₁›) { ‹t› } else { ‹f› }] [TF| test (‹c₂›) { ‹t› } else { ‹f› }]
-        | shortCircuit {c t₁ t₂ f₁ f₂} (h₁: Eval t₁ t₂) (h₂: Eval f₁ f₂) (h₃: t₂ = f₂): Eval₁ [TF| test (‹c›) { ‹t₁› } else { ‹f₁› }] t₁
+        | shortCircuit {c t₁ t₂ f₁ f₂} (h₁: Eval₁ t₁ t₂) (h₂: Eval₁ f₁ f₂) (h₃: t₂ = f₂): Eval₁ [TF| test (‹c›) { ‹t₁› } else { ‹f₁› }] t₁
 
       notation t₁ "⟶" t₂ => Eval₁ t₁ t₂
 
@@ -511,5 +543,509 @@ namespace SoftwareFoundations.ProgrammingLanguageFoundations.SmallStep
   ## Multi-Step Reduction
   -/
 
+  inductive MultiStep (R: Relation α): Relation α where
+    | refl {x: α}: MultiStep R x x
+    | step {x₁ x₂ x₃: α} (h₁: R x₁ x₂) (h₂: MultiStep R x₂ x₃): MultiStep R x₁ x₃
 
+  -- Allows the use of `calc` proofs
+  instance (R: Relation α): Trans R R (MultiStep R) where
+    trans h₁ h₂ := .step h₁ (.step h₂ .refl)
+  instance: Trans R (MultiStep R) (MultiStep R) where
+    trans h₁ h₂ := .step h₁ h₂
+  instance: Trans (MultiStep R) R (MultiStep R) where
+    -- This can't be done term-style and has to be done with tactics because of
+    -- shortcomings in the Lean equation compiler.  See
+    -- [this GitHub issue](https://github.com/leanprover/lean4/pull/1672)
+    trans h₁ h₂ := by
+      induction h₁ with
+        | refl =>
+          apply MultiStep.step
+          · exact h₂
+          · apply MultiStep.refl
+        | step h₁ _ ih =>
+          apply MultiStep.step
+          · exact h₁
+          · apply ih
+            · exact h₂
+  instance: Trans (MultiStep R) (MultiStep R) (MultiStep R) where
+    -- This can't be done term-style and has to be done with tactics because of
+    -- shortcomings in the Lean equation compiler.  See
+    -- [this GitHub issue](https://github.com/leanprover/lean4/pull/1672)
+    trans h₁ h₂ := by
+      induction h₁ with
+        | refl => exact h₂
+        | step h₁ _ ih =>
+          apply MultiStep.step
+          · exact h₁
+          · apply ih
+            · exact h₂
+
+  notation t₁ "↠" t₂ => MultiStep Eval₁ t₁ t₂
+  infix:50 "⇒" => Eval₁
+
+  namespace Term
+    theorem MultiStep.contains_R {R: Relation α} {x₁ x₂: α}: R x y → MultiStep R x y
+      | h => .step h .refl
+
+    -- This can't be done term-style and has to be done with tactics because of
+    -- shortcomings in the Lean equation compiler.  See
+    -- [this GitHub issue](https://github.com/leanprover/lean4/pull/1672)
+    theorem MultiStep.transitive {R: Relation α} {x₁ x₂ x₃: α}: MultiStep R x₁ x₂ → MultiStep R x₂ x₃ → MultiStep R x₁ x₃ := sorry
+  end Term
+
+  namespace Tactic
+    theorem MultiStep.contains_R {R: Relation α} {x₁ x₂: α} (h: R x y): MultiStep R x y := by
+      apply MultiStep.step
+      · exact h
+      · apply MultiStep.refl
+
+    theorem MultiStep.transitive {R: Relation α} {x₁ x₂ x₃: α} (h₁: MultiStep R x₁ x₂) (h₂: MultiStep R x₂ x₃): MultiStep R x₁ x₃ := by
+      induction h₁ with
+        | refl => exact h₂
+        | step h₁ _ ih =>
+          apply MultiStep.step
+          · exact h₁
+          · apply ih
+            · exact h₂
+  end Tactic
+
+  namespace Blended
+    theorem MultiStep.contains_R {R: Relation α} {x₁ x₂: α}: R x y → MultiStep R x y
+      | h => .step h .refl
+
+    -- This can't be done term-style and has to be done with tactics because of
+    -- shortcomings in the Lean equation compiler.  See
+    -- [this GitHub issue](https://github.com/leanprover/lean4/pull/1672)
+    theorem MultiStep.transitive {R: Relation α} {x₁ x₂ x₃: α}: MultiStep R x₁ x₂ → MultiStep R x₂ x₃ → MultiStep R x₁ x₃ := sorry
+  end Blended
+
+  /-
+  ### Examples
+  -/
+
+  namespace Term
+    example: [Toy| (0 + 3) + (2 + 4)] ↠ [Toy| ‹(0 + 3) + (2 + 4)›] :=
+      calc [Toy| (0 + 3) + (2 + 4)]
+        _ ⇒ [Toy| 3 + (2 + 4)] := .plusL .constConst
+        _ ⇒ [Toy| 3 + 6]       := .plusR (.const 3) .constConst
+        _ ⇒ [Toy| 9]           := .constConst
+
+    example: [Toy| 3]     ↠ [Toy| 3]     := .refl
+    example: [Toy| 0 + 3] ↠ [Toy| 0 + 3] := .refl
+
+    example: [Toy| 0 + (2 + (0 + 3))] ↠ [Toy| 0 + ‹2 + (0 + 3)›] :=
+      calc [Toy| 0 + (2 + (0 + 3))]
+        _ ⇒ [Toy| 0 + (2 + 3)] := .plusR (.const 0) (.plusR (.const 2) .constConst)
+        _ ⇒ [Toy| 0 + 5]       := .plusR (.const 0) .constConst
+  end Term
+
+  namespace Tactic
+    example: [Toy| (0 + 3) + (2 + 4)] ↠ [Toy| ‹(0 + 3) + (2 + 4)›] := by
+      apply MultiStep.step
+      · apply Eval₁.plusL
+        · apply Eval₁.constConst
+      · apply MultiStep.step
+        · apply Eval₁.plusR
+          . apply Value.const
+          · apply Eval₁.constConst
+        · apply MultiStep.step
+          · apply Eval₁.constConst
+          . apply MultiStep.refl
+
+    example: [Toy| 3] ↠ [Toy| 3] := by
+      apply MultiStep.refl
+
+    example: [Toy| 0 + 3] ↠ [Toy| 0 + 3] := by
+      apply MultiStep.refl
+
+    example: [Toy| 0 + (2 + (0 + 3))] ↠ [Toy| 0 + ‹2 + (0 + 3)›] := by
+      apply MultiStep.step
+      · apply Eval₁.plusR
+        · apply Value.const
+        · apply Eval₁.plusR
+          · apply Value.const
+          · apply Eval₁.constConst
+      · apply MultiStep.step
+        · apply Eval₁.plusR
+          · apply Value.const
+          · apply Eval₁.constConst
+        · apply MultiStep.refl
+  end Tactic
+
+  namespace Blended
+    example: [Toy| (0 + 3) + (2 + 4)] ↠ [Toy| ‹(0 + 3) + (2 + 4)›] :=
+      calc [Toy| (0 + 3) + (2 + 4)]
+        _ ⇒ [Toy| 3 + (2 + 4)] := .plusL .constConst
+        _ ⇒ [Toy| 3 + 6]       := .plusR (.const 3) .constConst
+        _ ⇒ [Toy| 9]           := .constConst
+
+    example: [Toy| 3]     ↠ [Toy| 3]     := .refl
+    example: [Toy| 0 + 3] ↠ [Toy| 0 + 3] := .refl
+
+    example: [Toy| 0 + (2 + (0 + 3))] ↠ [Toy| 0 + ‹2 + (0 + 3)›] :=
+      calc [Toy| 0 + (2 + (0 + 3))]
+        _ ⇒ [Toy| 0 + (2 + 3)] := .plusR (.const 0) (.plusR (.const 2) .constConst)
+        _ ⇒ [Toy| 0 + 5]       := .plusR (.const 0) .constConst
+  end Blended
+
+  /-
+  ### Normal Forms, Again
+  -/
+
+  def Eval₁.normal: Term → Prop := Relation.normal Eval₁
+
+  def Term.normalOf (t₁ t₂: Term): Prop := Eval₁ t₂ t₁ ∧ Eval₁.normal t₁
+
+  namespace Term
+    theorem Eval₁.normal.unique: Relation.deterministic Term.normalOf
+      | t₁, t₂, t₃, ⟨he₁, hn₁⟩, ⟨he₂, hn₂⟩ =>
+        have h₃: t₂ = t₁ :=
+          calc t₂
+            _ ⇒ t₁ := he₁
+            _ = t₁ := sorry
+        have h₄: t₃ = t₁ :=
+          calc t₃
+            _ ⇒ t₁ := he₂
+            _ = t₁ := sorry
+        calc t₂
+          _ = t₁ := h₃
+          _ = t₃ := Eq.symm h₄
+  end Term
+
+  namespace Tactic
+    theorem Eval₁.normal.unique: Relation.deterministic Term.normalOf := by sorry
+  end Tactic
+
+  namespace Blended
+    theorem Eval₁.normal.unique: Relation.deterministic Term.normalOf
+      | t₁, t₂, t₃, h₁, h₂ =>
+        have h₃ :=
+          calc t₂
+            _ = t₁ := sorry
+        have h₄ :=
+          calc t₃
+            _ = t₁ := sorry
+        by rw [h₃, h₄]
+  end Blended
+
+  def Relation.normalizing (R: Relation α): Prop := ∀ t₁: α, ∃ t₂: α, MultiStep R t₁ t₂ ∧ Relation.normal R t₂
+
+  namespace Term
+    theorem Eval₁.normalizing: Relation.normalizing Eval₁
+      | .const n =>
+        have hn := Value.normal (.const n)
+        ⟨[Toy| ‹n›], ⟨.refl, hn⟩⟩
+      | .plus t₁ t₂ =>
+        have ⟨nt₁, ⟨w₁, hw₁⟩⟩ := normalizing t₁
+        have ⟨nt₂, ⟨w₂, hw₂⟩⟩ := normalizing t₂
+        match nt₁, nt₂ with
+          | .const n₁, const n₂ => sorry
+          | _, _ => sorry
+      where
+        plusL_normalizing (t₁ t₂ t₃: Term) (h: Eval₁ t₁ t₂): Eval₁ [Toy| ‹‹t₁›› + ‹‹t₃››] [Toy| ‹‹t₂›› + ‹‹t₃››] := sorry
+        plusR_normalizing (v₁ t₁ t₂: Term) (h₁: Value v₁) (h₂: Eval₁ t₁ t₂): Eval₁ [Toy| ‹‹v₁›› + ‹‹t₁››] [Toy| ‹‹v₁›› + ‹‹t₂››] := sorry
+  end Term
+
+  namespace Tactic
+    theorem Eval₁.normalizing: Relation.normalizing Eval₁ := by
+      sorry
+      where
+        plusL_normalizing (t₁ t₂ t₃: Term) (h: Eval₁ t₁ t₂): Eval₁ [Toy| ‹‹t₁›› + ‹‹t₃››] [Toy| ‹‹t₂›› + ‹‹t₃››] := by sorry
+        plusR_normalizing (v₁ t₁ t₂: Term) (h₁: Value v₁) (h₂: Eval₁ t₁ t₂): Eval₁ [Toy| ‹‹v₁›› + ‹‹t₁››] [Toy| ‹‹v₁›› + ‹‹t₂››] := by sorry
+  end Tactic
+
+  namespace Blended
+    theorem Eval₁.normalizing: Relation.normalizing Eval₁ :=
+      sorry
+      where
+        plusL_normalizing (t₁ t₂ t₃: Term) (h: Eval₁ t₁ t₂): Eval₁ [Toy| ‹‹t₁›› + ‹‹t₃››] [Toy| ‹‹t₂›› + ‹‹t₃››] := sorry
+        plusR_normalizing (v₁ t₁ t₂: Term) (h₁: Value v₁) (h₂: Eval₁ t₁ t₂): Eval₁ [Toy| ‹‹v₁›› + ‹‹t₁››] [Toy| ‹‹v₁›› + ‹‹t₂››] := sorry
+  end Blended
+
+  /-
+  ### Equivalence of Big-Step and Small-Step
+  -/
+
+  namespace Term
+    theorem Eval₁.equiv_multistep (t: Term) (n: Nat): t.eval == n → MultiStep Eval₁ t [Toy| ‹n›]
+      | h => sorry
+  end Term
+
+  /-
+  ### Additional Exercises
+  -/
+
+  namespace Combined
+    inductive Term: Type where
+      | const (n: Nat): Term
+      | plus (t₁ t₂: Term): Term
+      | true: Term
+      | false: Term
+      | test: Term → Term → Term → Term
+
+    declare_syntax_cat combined
+
+    syntax num : combined
+    syntax "tru" : combined
+    syntax "fls" : combined
+    syntax:max "‹nat:" term "›" : combined
+    syntax:max "‹bool:" term "›" : combined
+    syntax:max "‹‹" term "››" : combined
+    syntax:60 combined:60 "+" combined:61 : combined
+    syntax "test" "(" combined ")" "{" combined "}" "else" "{" combined "}" : combined
+    syntax "(" combined ")" : combined
+
+    syntax "[Combined|" combined "]" : term
+
+    macro_rules
+      | `([Combined| tru])                            => `(Term.true)
+      | `([Combined| fls])                            => `(Term.true)
+      | `([Combined| ‹nat: $n:term ›])                => `(Term.const $(Lean.quote n))
+      | `([Combined| ‹bool: true ›])                  => `(Term.true)
+      | `([Combined| ‹bool: false ›])                 => `(Term.false)
+      | `([Combined| ‹‹ $t:term ›› ])                 => `($(Lean.quote t))
+      | `([Combined| $t₁ + $t₂])                      => `(Term.plus [Combined| $t₁] [Combined| $t₂])
+      | `([Combined| test ( $c ) { $t } else { $f }]) => `(Term.test [Combined| $c] [Combined| $t] [Combined| $f])
+      | `([Combined| ( $t )])                         => `([Combined| $t])
+
+    inductive Value: Term → Prop where
+      | true: Value [Combined| tru]
+      | false: Value [Combined| fls]
+      | const (n: Nat): Value [Combined| ‹nat:n›]
+
+    inductive Eval₁: Term → Term → Prop where
+      | constConst {n₁ n₂: Nat}: Eval₁ [Combined| ‹nat:n₁› + ‹nat:n₂›] [Combined| ‹nat:n₁ + n₂›]
+      | plusL {t₁ t₂ t₃: Term} (h₁: Eval₁ t₁ t₂): Eval₁ [Combined| ‹‹t₁›› + ‹‹t₃››] [Combined| ‹‹t₂›› + ‹‹t₃››]
+      | plusR {v₁ t₁ t₂: Term} (h₁: Value v₁) (h₂: Eval₁ t₁ t₂): Eval₁ [Combined| ‹‹v₁›› + ‹‹t₁››] [Combined| ‹‹v₁›› + ‹‹t₂››]
+      | testTrue {t f: Term}: Eval₁ [Combined| test (tru) { ‹‹t›› } else { ‹‹f›› }] [Combined| ‹‹t››]
+      | testFalse {t f: Term}: Eval₁ [Combined| test (fls) { ‹‹t›› } else { ‹‹f›› }] [Combined| ‹‹f››]
+      | test {c₁ c₂ t f: Term} (h₁: Eval₁ c₁ c₂): Eval₁ [Combined| test (‹‹c₁››) { ‹‹t›› } else { ‹‹f›› }] [Combined| test (‹‹c₂››) { ‹‹t›› } else { ‹‹f›› }]
+
+    namespace Term
+      theorem Eval₁.deterministic: Relation.deterministic Eval₁ := sorry
+      theorem Eval₁.strong_progress: ((t₁: Term) → Value t₁ ∨ ∃ t₂: Term, Eval₁ t₁ t₂) ∨ ¬((t₁: Term) → Value t₁ ∨ ∃ t₂: Term, Eval₁ t₁ t₂) := sorry
+    end Term
+
+    namespace Tactic
+      theorem Eval₁.deterministic: Relation.deterministic Eval₁ := by sorry
+      theorem Eval₁.strong_progress: ((t₁: Term) → Value t₁ ∨ ∃ t₂: Term, Eval₁ t₁ t₂) ∨ ¬((t₁: Term) → Value t₁ ∨ ∃ t₂: Term, Eval₁ t₁ t₂) := by sorry
+    end Tactic
+
+    namespace Blended
+      theorem Eval₁.deterministic: Relation.deterministic Eval₁ := sorry
+      theorem Eval₁.strong_progress: ((t₁: Term) → Value t₁ ∨ ∃ t₂: Term, Eval₁ t₁ t₂) ∨ ¬((t₁: Term) → Value t₁ ∨ ∃ t₂: Term, Eval₁ t₁ t₂) := sorry
+    end Blended
+  end Combined
+
+  /-
+  ## Small-Step Imp
+  -/
+
+  open Imp
+
+  abbrev State := _root_.SoftwareFoundations.LogicalFoundations.Imp.State
+  abbrev Arith := _root_.SoftwareFoundations.LogicalFoundations.Imp.Arith
+  abbrev Logic := _root_.SoftwareFoundations.LogicalFoundations.Imp.Logic
+  abbrev Command := _root_.SoftwareFoundations.LogicalFoundations.Imp.Command
+
+  inductive ArithValue: Arith → Prop where
+    | const (n: Nat): ArithValue [Arith| ‹num:n›]
+
+  inductive LogicValue: Logic → Prop where
+    | true: LogicValue [Logic| tru]
+    | false: LogicValue [Logic| fls]
+
+  inductive ArithEval₁ (s: State): Arith → Arith → Prop where
+    | ident {id: String}: ArithEval₁ s [Arith| ‹id:id›] [Arith| ‹num:(s id)›]
+    | plusL {e₁ e₂ e₃: Arith} (h₁: ArithEval₁ s e₁ e₂): ArithEval₁ s [Arith| ‹e₁› + ‹e₃›] [Arith| ‹e₂› + ‹e₃›]
+    | plusR {v₁ e₁ e₂: Arith} (h₁: ArithValue v₁) (h₂: ArithEval₁ s e₁ e₂): ArithEval₁ s [Arith| ‹v₁› + ‹e₁›] [Arith| ‹v₁› + ‹e₂›]
+    | plus {v₁ v₂: Nat}: ArithEval₁ s [Arith| ‹num:v₁› + ‹num:v₂›] [Arith| ‹num:v₁ + v₂›]
+    | minusL {e₁ e₂ e₃: Arith} (h₁: ArithEval₁ s e₁ e₂): ArithEval₁ s [Arith| ‹e₁› - ‹e₃›] [Arith| ‹e₂› - ‹e₃›]
+    | minusR {v₁ e₁ e₂: Arith} (h₁: ArithValue v₁) (h₂: ArithEval₁ s e₁ e₂): ArithEval₁ s [Arith| ‹v₁› - ‹e₁›] [Arith| ‹v₁› - ‹e₂›]
+    | minus {v₁ v₂: Nat}: ArithEval₁ s [Arith| ‹num:v₁› - ‹num:v₂›] [Arith| ‹num:v₁ - v₂›]
+    | multL {e₁ e₂ e₃: Arith} (h₁: ArithEval₁ s e₁ e₂): ArithEval₁ s [Arith| ‹e₁› * ‹e₃›] [Arith| ‹e₂› * ‹e₃›]
+    | multR {v₁ e₁ e₂: Arith} (h₁: ArithValue v₁) (h₂: ArithEval₁ s e₁ e₂): ArithEval₁ s [Arith| ‹v₁› * ‹e₁›] [Arith| ‹v₁› * ‹e₂›]
+    | mult {v₁ v₂: Nat}: ArithEval₁ s [Arith| ‹num:v₁› * ‹num:v₂›] [Arith| ‹num:v₁ * v₂›]
+
+  inductive LogicEval₁ (s: State): Logic → Logic → Prop where
+    | eqL {e₁ e₂ e₃: Arith} (h₁: ArithEval₁ s e₁ e₂): LogicEval₁ s [Logic| ‹e₁› = ‹e₃›] [Logic| ‹e₂› = ‹e₃›]
+    | eqR {v₁ e₁ e₂: Arith} (h₁: ArithEval₁ s e₁ e₂): LogicEval₁ s [Logic| ‹v₁› = ‹e₁›] [Logic| ‹v₁› = ‹e₂›]
+    | eq {v₁ v₂: Nat}: LogicEval₁ s [Logic| ‹num:v₁› = ‹num:v₂›] [Logic| ‹‹v₁ == v₂››]
+    | neqL {e₁ e₂ e₃: Arith} (h₁: ArithEval₁ s e₁ e₂): LogicEval₁ s [Logic| ‹e₁› ≠ ‹e₃›] [Logic| ‹e₂› ≠ ‹e₃›]
+    | neqR {v₁ e₁ e₂: Arith} (h₁: ArithValue v₁) (h₂: ArithEval₁ s e₁ e₂): LogicEval₁ s [Logic| ‹v₁› ≠ ‹e₁›] [Logic| ‹v₁› ≠ ‹e₂›]
+    | neq {v₁ v₂: Nat}: LogicEval₁ s [Logic| ‹num:v₁› ≠ ‹num:v₂›] [Logic| ‹‹v₁ != v₂››]
+    | leL {e₁ e₂ e₃: Arith} (h₁: ArithEval₁ s e₁ e₂): LogicEval₁ s [Logic| ‹e₁› ≤ ‹e₃›] [Logic| ‹e₂› ≤ ‹e₃›]
+    | leR {v₁ e₁ e₂: Arith} (h₁: ArithValue v₁) (h₂: ArithEval₁ s e₁ e₂): LogicEval₁ s [Logic| ‹v₁› ≤ ‹e₁›] [Logic| ‹v₁› ≤ ‹e₂›]
+    | le {v₁ v₂: Nat}: LogicEval₁ s [Logic| ‹num:v₁› ≤ ‹num:v₂›] [Logic| ‹‹v₁ ≤ v₂››]
+    | gtL {e₁ e₂ e₃: Arith} (h₁: ArithEval₁ s e₁ e₂): LogicEval₁ s [Logic| ‹e₁› > ‹e₃›] [Logic| ‹e₂› > ‹e₃›]
+    | gtR {v₁ e₁ e₂: Arith} (h₁: ArithValue v₁) (h₂: ArithEval₁ s e₁ e₂): LogicEval₁ s [Logic| ‹v₁› > ‹e₁›] [Logic| ‹v₁› > ‹e₂›]
+    | gt {v₁ v₂: Nat}: LogicEval₁ s [Logic| ‹num:v₁› > ‹num:v₂›] [Logic| ‹‹v₁ > v₂››]
+    | notTrue: LogicEval₁ s [Logic| ! tru] [Logic| fls]
+    | notFalse: LogicEval₁ s [Logic| ! fls] [Logic| tru]
+    | not {b₁ b₂: Logic} (h₁: LogicEval₁ s b₁ b₂): LogicEval₁ s [Logic| ‹b₁›] [Logic| ‹b₂›]
+    | andL {b₁ b₂ b₃: Logic} (h₁: LogicEval₁ s b₁ b₂): LogicEval₁ s [Logic| ‹b₁› && ‹b₃›] [Logic| ‹b₂› && ‹b₃›]
+    | andR {v₁ b₁ b₂: Logic} (h₁: LogicValue v₁) (h₂: LogicEval₁ s b₁ b₂): LogicEval₁ s [Logic| ‹v₁› && ‹b₁›] [Logic| ‹v₁› && ‹b₂›]
+    | and {v₁ v₂: Bool}: LogicEval₁ s [Logic| ‹‹v₁›› && ‹‹v₂››] [Logic| ‹‹v₁ && v₂››]
+
+  inductive CommandEval₁: (Command × State) → (Command × State) → Prop where
+    | assignStep {s: State} {id: String} {e₁ e₂: Arith} (h₁: ArithEval₁ s e₁ e₂): CommandEval₁ ([Imp| ‹id› := ‹e₁›], s) ([Imp| ‹id› := ‹e₂›], s)
+    | assign {s: State} {id: String} {n: Nat}: CommandEval₁ ([Imp| ‹id› := ‹num:n›], s) ([Imp| skip], s.update id n)
+    | seqStep {s₁ s₂: State} {c₁ c₂ c₃: Command} (h₁: CommandEval₁ (c₁, s₁) (c₂, s₂)): CommandEval₁ ([Imp| ‹c₁›; ‹c₃›], s₁) ([Imp| ‹c₂›; ‹c₃›], s₂)
+    | seq {s: State} {c: Command}: CommandEval₁ ([Imp| skip; ‹c›], s) ([Imp| ‹c›], s)
+    | iteStep {s: State} {c₁ c₂: Logic} {t f: Command} (h₁: LogicEval₁ s c₁ c₂): CommandEval₁ ([Imp| ite (‹c₁›) { ‹t› } else { ‹f› }], s) ([Imp| ite (‹c₂›) { ‹t› } else { ‹f› }], s)
+    | iteTrue {s: State} {t f: Command}: CommandEval₁ ([Imp| ite (tru) { ‹t› } else { ‹f› }], s) ([Imp| ‹t›], s)
+    | iteFalse {s: State} {t f: Command}: CommandEval₁ ([Imp| ite (fls) { ‹t› } else { ‹f› }], s) ([Imp| ‹f›], s)
+    | while {s: State} {c: Logic} {b: Command}: CommandEval₁ ([Imp| while (‹c›) { ‹b› }], s) ([Imp| ite (‹c›) { ‹b›; while (‹c›) { ‹b› } } else { skip }], s)
+
+  /-
+  ## Concurrent Imp
+  -/
+
+  namespace ConcurrentImp
+    inductive Command: Type where
+      | skip: Command
+      | assign (id: String) (e: Arith): Command
+      | seq (c₁ c₂: Command): Command
+      | if (c: Logic) (t f: Command): Command
+      | while (c: Logic) (b: Command): Command
+      | parallel (c₁ c₂: Command): Command
+
+    declare_syntax_cat concurrent
+
+    syntax:50 "skip" : concurrent
+    syntax:50 ident ":=" arith : concurrent
+    syntax:50 "‹" term "›" ":=" arith : concurrent
+    syntax:40 concurrent ";" concurrent : concurrent
+    syntax:50 "ite" "(" logic ")" "{" concurrent "}" "else" "{" concurrent "}" : concurrent
+    syntax:50 "while" "(" logic ")" "{" concurrent "}" : concurrent
+    syntax:40 concurrent "||" concurrent : concurrent
+    syntax "(" concurrent ")" : concurrent
+    syntax "‹" term "›" : concurrent
+
+    syntax "[Concurrent|" concurrent "]" : term
+
+    macro_rules
+      | `([Concurrent| skip])                                => `(Command.skip)
+      | `([Concurrent| $id:ident := $e:arith])               => `(Command.assign $(Lean.quote (toString id.getId)) [Arith| $e])
+      | `([Concurrent| ‹$t:term› := $e:arith])               => `(Command.assign $(Lean.quote t) [Arith| $e])
+      | `([Concurrent| $x; $y])                              => `(Command.seq [Concurrent| $x] [Concurrent| $y])
+      | `([Concurrent| ite ( $c:logic ) { $t } else { $f }]) => `(Command.if [Logic| $c] [Concurrent| $t] [Concurrent| $f])
+      | `([Concurrent| while ( $c:logic ) { $b }])           => `(Command.while [Logic| $c] [Concurrent| $b])
+      | `([Concurrent| $c₁ || $c₂])                          => `(Command.parallel [Concurrent| $c₁] [Concurrent| $c₂])
+      | `([Concurrent| ( $c )])                              => `([Concurrent| $c])
+      | `([Concurrent| ‹$t:term› ])                          => pure t
+
+    inductive CommandEval₁: (Command × State) → (Command × State) → Prop where
+      | assignStep {s: State} {id: String} {e₁ e₂: Arith} (h₁: ArithEval₁ s e₁ e₂): CommandEval₁ ([Concurrent| ‹id› := ‹e₁›], s) ([Concurrent| ‹id› := ‹e₂›], s)
+      | assign {s: State} {id: String} {n: Nat}: CommandEval₁ ([Concurrent| ‹id› := ‹num:n›], s) ([Concurrent| skip], s.update id n)
+      | seqStep {s₁ s₂: State} {c₁ c₂ c₃: Command} (h₁: CommandEval₁ (c₁, s₁) (c₂, s₂)): CommandEval₁ ([Concurrent| ‹c₁›; ‹c₃›], s₁) ([Concurrent| ‹c₂›; ‹c₃›], s₂)
+      | seq {s: State} {c: Command}: CommandEval₁ ([Concurrent| skip; ‹c›], s) ([Concurrent| ‹c›], s)
+      | iteStep {s: State} {c₁ c₂: Logic} {t f: Command} (h₁: LogicEval₁ s c₁ c₂): CommandEval₁ ([Concurrent| ite (‹c₁›) { ‹t› } else { ‹f› }], s) ([Concurrent| ite (‹c₂›) { ‹t› } else { ‹f› }], s)
+      | iteTrue {s: State} {t f: Command}: CommandEval₁ ([Concurrent| ite (tru) { ‹t› } else { ‹f› }], s) ([Concurrent| ‹t›], s)
+      | iteFalse {s: State} {t f: Command}: CommandEval₁ ([Concurrent| ite (fls) { ‹t› } else { ‹f› }], s) ([Concurrent| ‹f›], s)
+      | while {s: State} {c: Logic} {b: Command}: CommandEval₁ ([Concurrent| while (‹c›) { ‹b› }], s) ([Concurrent| ite (‹c›) { ‹b›; while (‹c›) { ‹b› } } else { skip }], s)
+      | parallelL {s₁ s₂: State} {c₁ c₂ c₃: Command} (h₁: CommandEval₁ (c₁, s₁) (c₂, s₂)): CommandEval₁ ([Concurrent| ‹c₁› || ‹c₃›], s₁) ([Concurrent| ‹c₂› || ‹c₃›], s₂)
+      | parallelR {s₁ s₂: State} {c₁ c₂ c₃: Command} (h₁: CommandEval₁ (c₁, s₁) (c₂, s₂)): CommandEval₁ ([Concurrent| ‹c₃› || ‹c₁›], s₁) ([Concurrent| ‹c₃› || ‹c₂›], s₂)
+      | parallel {s: State}: CommandEval₁ ([Concurrent| skip || skip], s) ([Concurrent| skip], s)
+
+    def parallelLoop := [Concurrent|
+      Y := 1 || while (Y = 0) { X := X + 1 }
+    ]
+
+    instance: Trans CommandEval₁ CommandEval₁ CommandEval₁ where
+      trans hxy hyz := sorry
+
+    infix:50 "⤳" => CommandEval₁
+
+    example: ∃ s: State, CommandEval₁ (parallelLoop, [State|]) ([Concurrent| skip], s) ∧ s "X" = 0 :=
+      have hw :=
+        calc (parallelLoop, [State|])
+          _ ⤳ ([Concurrent| skip || while (Y = 0) { X := X + 1 }],                                           [State| Y = 1]) := .parallelL .assign
+          _ ⤳ ([Concurrent| skip || ite (Y = 0) { X := X + 1; while (Y = 0) { X := X + 1 } } else { skip }], [State| Y = 1]) := .parallelR .while
+          _ ⤳ ([Concurrent| skip || ite (1 = 0) { X := X + 1; while (Y = 0) { X := X + 1 } } else { skip }], [State| Y = 1]) := .parallelR (.iteStep (.eqL .ident))
+          _ ⤳ ([Concurrent| skip || ite (fls) { X := X + 1; while (Y = 0) { X := X + 1 } } else { skip }],   [State| Y = 1]) := .parallelR (.iteStep .eq)
+          _ ⤳ ([Concurrent| skip || skip],                                                                   [State| Y = 1]) := .parallelR .iteFalse
+          _ ⤳ ([Concurrent| skip],                                                                           [State| Y = 1]) := .parallel
+      ⟨[State| Y = 1], ⟨hw, rfl⟩⟩
+
+    example: ∃ s: State, CommandEval₁ (parallelLoop, [State|]) ([Concurrent| skip], s) ∧ s "X" = 2 :=
+      have hw :=
+        calc (parallelLoop, [State|])
+          _ ⤳ ([Concurrent| Y := 1 || ite (Y = 0) { X := X + 1; while (Y = 0) { X := X + 1 } } else { skip }], [State|])                     := .parallelR .while
+          _ ⤳ ([Concurrent| Y := 1 || ite (0 = 0) { X := X + 1; while (Y = 0) { X := X + 1 } } else { skip }], [State|])                     := .parallelR (.iteStep (.eqL .ident))
+          _ ⤳ ([Concurrent| Y := 1 || ite (tru) { X := X + 1; while (Y = 0) { X := X + 1 } } else { skip }],   [State|])                     := .parallelR (.iteStep .eq)
+          _ ⤳ ([Concurrent| Y := 1 || X := X + 1; while (Y = 0) { X := X + 1 }],                               [State|])                     := .parallelR .iteTrue
+          _ ⤳ ([Concurrent| Y := 1 || X := 0 + 1; while (Y = 0) { X := X + 1 }],                               [State|])                     := .parallelR (.seqStep (.assignStep (.plusL .ident)))
+          _ ⤳ ([Concurrent| Y := 1 || X := 1; while (Y = 0) { X := X + 1 }],                                   [State|])                     := .parallelR (.seqStep (.assignStep .plus))
+          _ ⤳ ([Concurrent| Y := 1 || skip; while (Y = 0) { X := X + 1 }],                                     [State| X = 1])               := .parallelR (.seqStep .assign)
+          _ ⤳ ([Concurrent| Y := 1 || while (Y = 0) { X := X + 1 }],                                           [State| X = 1])               := .parallelR .seq
+          _ ⤳ ([Concurrent| Y := 1 || ite (Y = 0) { X := X + 1; while (Y = 0) { X := X + 1 } } else { skip }], [State| X = 1])               := .parallelR .while
+          _ ⤳ ([Concurrent| Y := 1 || ite (0 = 0) { X := X + 1; while (Y = 0) { X := X + 1 } } else { skip }], [State| X = 1])               := .parallelR (.iteStep (.eqL .ident))
+          _ ⤳ ([Concurrent| skip || ite (0 = 0) { X := X + 1; while (Y = 0) { X := X + 1 } } else { skip }],   [State| X = 1, Y = 1])        := .parallelL .assign
+          _ ⤳ ([Concurrent| skip || ite (tru) { X := X + 1; while (Y = 0) { X := X + 1 } } else { skip }],     [State| X = 1, Y = 1])        := .parallelR (.iteStep .eq)
+          _ ⤳ ([Concurrent| skip || X := X + 1; while (Y = 0) { X := X + 1 }],                                 [State| X = 1, Y = 1])        := .parallelR .iteTrue
+          _ ⤳ ([Concurrent| skip || X := 1 + 1; while (Y = 0) { X := X + 1 }],                                 [State| X = 1, Y = 1])        := .parallelR (.seqStep (.assignStep (.plusL .ident)))
+          _ ⤳ ([Concurrent| skip || X := 2; while (Y = 0) { X := X + 1 }],                                     [State| X = 1, Y = 1])        := .parallelR (.seqStep (.assignStep .plus))
+          _ ⤳ ([Concurrent| skip || skip; while (Y = 0) { X := X + 1 }],                                       [State| X = 1, Y = 1, X = 2]) := .parallelR (.seqStep .assign)
+          _ ⤳ ([Concurrent| skip || while (Y = 0) { X := X + 1 }],                                             [State| X = 1, Y = 1, X = 2]) := .parallelR .seq
+          _ ⤳ ([Concurrent| skip || ite (Y = 0) { X := X + 1; while (Y = 0) { X := X + 1 } } else { skip }],   [State| X = 1, Y = 1, X = 2]) := .parallelR .while
+          _ ⤳ ([Concurrent| skip || ite (1 = 0) { X := X + 1; while (Y = 0) { X := X + 1 } } else { skip }],   [State| X = 1, Y = 1, X = 2]) := .parallelR (.iteStep (.eqL .ident))
+          _ ⤳ ([Concurrent| skip || ite (fls) { X := X + 1; while (Y = 0) { X := X + 1 } } else { skip }],     [State| X = 1, Y = 1, X = 2]) := .parallelR (.iteStep .eq)
+          _ ⤳ ([Concurrent| skip || skip],                                                                     [State| X = 1, Y = 1, X = 2]) := .parallelR .iteFalse
+          _ ⤳ ([Concurrent| skip],                                                                             [State| X = 1, Y = 1, X = 2]) := .parallel
+      ⟨[State| X = 1, Y = 1, X = 2], ⟨hw, rfl⟩⟩
+
+    namespace Term
+      theorem parallelLoop.any: ∀ n: Nat, ∃ s: State, CommandEval₁ (parallelLoop, [State|]) ([Concurrent| skip], s) ∧ s "X" = n
+        | .zero => sorry
+        | .succ n => sorry
+    end Term
+
+    namespace Tactic
+      theorem parallelLoop.any (n: Nat): ∃ s: State, CommandEval₁ (parallelLoop, [State|]) ([Concurrent| skip], s) ∧ s "X" = n := by
+        cases n with
+          | zero => sorry
+          | succ n => sorry
+    end Tactic
+
+    namespace Blended
+      theorem parallelLoop.any: ∀ n: Nat, ∃ s: State, CommandEval₁ (parallelLoop, [State|]) ([Concurrent| skip], s) ∧ s "X" = n
+        | .zero => sorry
+        | .succ n => sorry
+    end Blended
+  end ConcurrentImp
+
+  /-
+  ## A Small-Step Stack Machine
+  -/
+
+  abbrev Stack := _root_.SoftwareFoundations.LogicalFoundations.Imp.Stack
+  abbrev Program := _root_.SoftwareFoundations.LogicalFoundations.Imp.Program
+
+  inductive ProgramEval₁ (s: State): (Program × Stack) → (Program × Stack) → Prop where
+    | push {stk: Stack} {n: Nat} {p: Program}: ProgramEval₁ s (.push n :: p, stk) (p, n :: stk)
+    | load {stk: Stack} {id: String} {p: Program}: ProgramEval₁ s (.load id :: p, stk) (p, s id :: stk)
+    | plus {stk: Stack} {n₁ n₂: Nat} {p: Program}: ProgramEval₁ s (.plus :: p, n₂ :: n₁ :: stk) (p, (n₁ + n₂) :: stk)
+    | minus {stk: Stack} {n₁ n₂: Nat} {p: Program}: ProgramEval₁ s (.plus :: p, n₂ :: n₁ :: stk) (p, (n₁ - n₂) :: stk)
+    | mult {stk: Stack} {n₁ n₂: Nat} {p: Program}: ProgramEval₁ s (.plus :: p, n₂ :: n₁ :: stk) (p, (n₁ * n₂) :: stk)
+
+  def ProgramEval (s: State) := MultiStep (ProgramEval₁ s)
+
+  namespace Term
+    theorem Arith.compile.correct: True := sorry
+  end Term
+
+  namespace Tactic
+    theorem Arith.compile.correct: True := by sorry
+  end Tactic
+
+  namespace Blended
+    theorem Arith.compile.correct: True := sorry
+  end Blended
+
+  /-
+  ## Aside: A `normalize` Tactic
+  -/
+
+  -- TODO: Tactics in Lean
 end SoftwareFoundations.ProgrammingLanguageFoundations.SmallStep
